steps_with_examples=["Okay, let's derive the equation (a+b)Â² = aÂ² + 2ab + bÂ². This falls under the topic of **Algebra**, specifically expanding binomials. ğŸ§®", '**Step 1: Understand the Square** ğŸ“\n(a+b)Â² means (a+b) multiplied by itself: (a+b) * (a+b).', '**Step 2: Apply the Distributive Property (also known as FOIL)** ğŸ’¡\nWe need to multiply each term in the first (a+b) with each term in the second (a+b).\n(a+b) * (a+b) = a*(a+b) + b*(a+b)', "**Step 3: Distribute 'a' and 'b'** â•\nNow, distribute 'a' over (a+b) and 'b' over (a+b):\na*(a+b) = a*a + a*b = aÂ² + ab\nb*(a+b) = b*a + b*b = ba + bÂ²", '**Step 4: Combine the Results** ğŸ¤\nSo, (a+b)*(a+b) = aÂ² + ab + ba + bÂ²', '**Step 5: Simplify** âœ¨\nSince ab is the same as ba, we can combine them:\naÂ² + ab + ba + bÂ² = aÂ² + ab + ab + bÂ² = aÂ² + 2ab + bÂ²', '**Conclusion:** Therefore, (a+b)Â² = aÂ² + 2ab + bÂ². ğŸ‰'] documentation_links=['https://www.mathsisfun.com/algebra/binomial-theorem.html', 'https://www.dummies.com/article/academics-the-arts/math/algebra/how-to-foil-method-for-multiplying-binomials-145498/'] youtube_tutorials=['https://www.youtube.com/watch?v=auF4HDPGzD0', 'https://www.youtube.com/watch?v=mkcgvQOuUE4']